Define insertion_sort, prove it correct

src/util/list.lean
@@ -145,3 +145,99 @@ begin
   simp [h_1] at x_notin,
   exact xs_ih x_notin a,
 end
+
+def ord_insert
+  {t: Type}
+  [linear_order t]
+  [decidable_rel ((≤): t -> t -> Prop)]
+  [is_trans t (≤)]
+  (x: t)
+: list t -> list t
+| [] := [x]
+| (y :: ys) := if x ≤ y then x :: y :: ys else y :: ord_insert ys
+
+def insertion_sort
+  {t: Type}
+  [linear_order t]
+  [decidable_rel ((≤): t -> t -> Prop)]
+  [is_trans t (≤)]
+: list t -> list t
+| [] := []
+| (x :: xs) := ord_insert x (insertion_sort xs)
+
+def sorted {t: Type} [preorder t]: list t -> Prop := pairwise (≤)
+
+theorem ord_insert_mem
+  {t: Type}
+  [linear_order t]
+  [decidable_rel ((≤): t -> t -> Prop)]
+  [is_trans t (≤)]
+  {x: t} {xs: list t}:
+  ∀ (y ∈ ord_insert x xs), y = x ∨ y ∈ xs :=
+begin
+  intros y h,
+  induction xs,
+  simp [ord_insert] at h,
+  exact or.inl h,
+  simp [ord_insert] at h,
+  cases decidable.em (x ≤ xs_hd),
+  simp [h_1] at h,
+  exact h,
+  simp [h_1] at h,
+  cases h,
+  right,
+  simp,
+  exact or.inl h,
+  cases xs_ih h,
+  exact or.inl h_2,
+  right,
+  simp,
+  exact or.inr h_2,
+end
+
+theorem ord_insert_spec
+  {t: Type}
+  [linear_order t]
+  [decidable_rel ((≤): t -> t -> Prop)]
+  [is_trans t (≤)]
+  (x: t) (xs: list t):
+  sorted xs -> sorted (ord_insert x xs) :=
+begin
+  intro h,
+  induction h,
+  simp [ord_insert],
+  exact pairwise.cons (list.ball_nil (fun y, x ≤ y)) (pairwise.nil (≤)),
+  simp [ord_insert],
+  cases decidable.em (x ≤ h_x),
+  simp [h],
+  let a: sorted (h_x :: h_xs) := pairwise.cons h_a h_a_1,
+  let b: ∀ (a: t), a ∈ h_x :: h_xs -> x ≤ a := fun a, fun b,
+    or.elim b
+    (fun b, begin rw b, exact h end)
+    (fun b, trans h (h_a a b)),
+  exact pairwise.cons b a,
+  simp [h],
+  let b: ∀ (a: t), a ∈ ord_insert x h_xs -> h_x ≤ a := fun a, fun b,
+  begin
+    cases ord_insert_mem a b,
+    rw h_1,
+    exact le_of_not_le h,
+    exact h_a a h_1,
+  end,
+  exact pairwise.cons b h_ih,
+end
+
+theorem insertion_sort_spec
+  {t: Type}
+  [linear_order t]
+  [decidable_rel ((≤): t -> t -> Prop)]
+  [is_trans t (≤)]
+  (xs: list t):
+  sorted (insertion_sort xs) :=
+begin
+  induction xs,
+  simp [insertion_sort],
+  exact pairwise.nil (≤),
+  simp [insertion_sort],
+  exact ord_insert_spec xs_hd (insertion_sort xs_tl) xs_ih,
+end
